Core/Metatheory/Global.lean
@@ -1,0 +1,580 @@
+
+import Core.Term
+import Core.Reduction
+import Core.Typing
+import Core.Global
+
+-- import Core.Metatheory.Substitution
+-- import Core.Metatheory.Rename
+-- import Core.Metatheory.Closed
+
+namespace Core
+
+
+theorem GlobalWf.drop_wf : ∀ n, ⊢ G -> ⊢ G.drop n := by
+  intro n wf
+  induction wf generalizing n
+  case _ => simp; constructor
+  case _ g gwf wf ih =>
+  induction n
+  case _ => simp; constructor; assumption; assumption
+  case _ => simp; apply ih
+
+-- theorem GlobalWf.drop_lookup_unique_vec :
+--   (∀ i, v i = none) ->
+--   Vect.fold (lookup x G) Option.or v = lookup x G
+-- := by
+--   intro h
+--   induction v using Vect.induction
+--   case _ => simp
+--   case _ hd tl ih =>
+--     simp; have lem := h 0; simp at lem
+--     subst lem; simp
+--     rw [ih]; intro i
+--     apply h (Fin.succ i)
+
+theorem GlobalWf.drop_lookup_unique {G : List Global} n :
+  ⊢ G ->
+  lookup x (G.drop n) = some t ->
+  lookup x G = some t
+:= by
+  sorry
+  -- intro wf j
+  -- induction wf generalizing n <;> simp at *
+  -- case nil => exact j
+  -- case cons G j1 j2 wf ih =>
+  --   cases n <;> simp at *
+  --   case zero => exact j
+  --   case succ n =>
+  --     replace ih := ih n j
+  --     cases j2
+  --     case data n y K ctors j1 j2 j3 =>
+  --       simp [lookup]; split
+  --       case _ e => subst e; rw [ih] at j3; injection j3
+  --       case _ e =>
+  --         rw [drop_lookup_unique_vec]; exact ih
+  --         intro i
+  --         generalize endef : ctors i = en at *
+  --         rcases en with ⟨z, A⟩; simp; intro e2; subst e2
+  --         replace j2 := j2 i x A endef
+  --         rcases j2 with ⟨q1, q2, q3, q4⟩
+  --         rw [ih] at q4; injection q4
+  --     case openm T b y j1 j2 =>
+  --       simp [lookup]; split
+  --       case _ e => subst e; rw [ih] at j2; injection j2
+  --       case _ e => exact ih
+  --     case opent y j1 j2 =>
+  --       simp [lookup]; split
+  --       case _ e => subst e; rw [ih] at j2; injection j2
+  --       case _ e => exact ih
+  --     case defn T b t' y j1 j2 j3 =>
+  --       simp [lookup]; split
+  --       case _ e => subst e; rw [ih] at j3; injection j3
+  --       case _ e => exact ih
+  --     case inst y T t' j1 j2 => simp [lookup]; exact ih
+  --     case instty y T j1 j2 =>
+  --       simp [lookup]; split
+  --       case _ e => subst e; rw [ih] at j2; injection j2
+  --       case _ e => exact ih
+
+theorem GlobalWf.drop_lookup_impossible {G : List Global} :
+  ⊢ G ->
+  G' = G.drop n ->
+  lookup x G' = some t ->
+  lookup x G = none ->
+  False
+:= by
+  intro wf e h1 h2
+  subst e; replace h1 := drop_lookup_unique n wf h1
+  rw [h2] at h1; injection h1
+
+theorem GlobalWf.drop_lookup {G : List Global} n :
+  ⊢ G ->
+  G' = G.drop n ->
+  lookup x G' = some t ->
+  lookup x G = some t' ->
+  t = t'
+:= by
+  sorry
+  -- intro wf e h1 h2
+  -- subst e; replace h1 := drop_lookup_unique n wf h1
+  -- have lem := Global.lookup_unique h1 h2
+  -- injection lem
+
+theorem Kinding.drop_weaken_global n :
+  ⊢ G ->
+  G' = G.drop n ->
+  G'& Δ ⊢ T : K ->
+  G&Δ ⊢ T : K
+:= by
+  intro wf e j
+  induction j generalizing G
+  case var =>
+    apply Kinding.var; assumption
+  case global x K Δ h =>
+    apply Kinding.global
+    simp [lookup_kind] at *;
+    generalize zdef  : lookup x G = z at *
+    generalize zdef' : lookup x G' = z' at *
+    cases z'; simp at h; case _ z' =>
+    cases z; simp at h
+    case none =>
+      exfalso
+      apply GlobalWf.drop_lookup_impossible wf e zdef' zdef
+    case some z =>
+      have lem := GlobalWf.drop_lookup n wf e zdef' zdef
+      subst z'; assumption
+  case all j ih =>
+    replace ih := @ih G wf e
+    apply Kinding.all; assumption
+  all_goals (case _ ih1 ih2 =>
+    replace ih1 := @ih1 G wf e
+    replace ih2 := @ih2 G wf e
+    constructor; assumption; assumption)
+
+theorem GlobalWf.drop_weaken_global_lookup_map (f : Entry -> Bool) n :
+  ⊢ G ->
+  G' = G.drop n ->
+  (Option.map f (lookup x G')).get! ->
+  (Option.map f (lookup x G)).get!
+:= by
+  intro wf e j
+  generalize zpdef : lookup x G' = z' at *
+  generalize zdef : lookup x G = z at *
+  cases z' <;> simp at j; case _ z' =>
+  cases z
+  case none =>
+    have lem := GlobalWf.drop_lookup_impossible wf e zpdef zdef
+    cases lem
+  case some z =>
+    have lem := GlobalWf.drop_lookup n wf e zpdef zdef; subst lem
+    simp; exact j
+
+
+theorem Typing.drop_weaken_global n :
+  ⊢ G ->
+  G' = G.drop n ->
+  G'&Δ,Γ ⊢ t : T ->
+  G&Δ,Γ ⊢ t : T
+:= by
+  sorry
+  -- intro wf e j
+  -- induction j generalizing G
+  -- case var j1 j2 =>
+  --   apply var j1
+  --   apply Kinding.drop_weaken_global n wf e j2
+  -- case global x A Δ b Γ j1 j2 =>
+  --   apply global _
+  --   apply Kinding.drop_weaken_global n wf e j2
+  --   simp [lookup_type] at *
+  --   generalize zdef  : lookup x G = z at *
+  --   generalize zdef' : lookup x G' = z' at *
+  --   cases z'; simp at j1; case _ z' =>
+  --   cases z; simp at j1
+  --   case none =>
+  --     exfalso
+  --     apply GlobalWf.drop_lookup_impossible wf e zdef' zdef
+  --   case some z =>
+  --     have lem := GlobalWf.drop_lookup n wf e zdef' zdef
+  --     subst z'; assumption
+  -- case mtch j1 j2 j3 j4 j5 j6 j7 j8 ih1 ih2 ih3 ih4 =>
+  --   apply mtch
+  --   apply ih1 wf e
+  --   apply ValidTyHeadVariable.drop_weaken_global_is_data n wf e j2
+  --   apply ih2 wf e
+  --   intro i; apply ValidHeadVariable.drop_weaken_global_is_ctor n wf e (j4 i)
+  --   intro i; apply ih3 i wf e
+  --   apply j6
+  --   intro i; apply ih4 i wf e
+  --   apply j8
+  -- case guard j1 j2 j3 j4 j5 j6 j7 ih1 ih2 ih3 =>
+  --   apply guard
+  --   apply ih1 wf e
+  --   apply ih2 wf e
+  --   apply ih3 wf e
+  --   apply ValidHeadVariable.drop_weaken_global_is_instty n wf e j4
+  --   apply ValidTyHeadVariable.drop_weaken_global_is_opent n wf e j5
+  --   apply j6
+  --   apply j7
+  -- case lam j1 j2 ih =>
+  --   apply lam
+  --   apply Kinding.drop_weaken_global n wf e j1
+  --   apply ih wf e
+  -- case app j1 j2 j3 ih1 ih2 =>
+  --   apply app
+  --   apply Kinding.drop_weaken_global n wf e j1
+  --   apply ih1 wf e
+  --   apply ih2 wf e
+  -- case lamt j1 j2 ih =>
+  --   apply lamt
+  --   apply Kinding.drop_weaken_global n wf e j1
+  --   apply ih wf e
+  -- case appt j1 j2 j3 ih =>
+  --   apply appt
+  --   apply ih wf e
+  --   apply Kinding.drop_weaken_global n wf e j2
+  --   apply j3
+  -- case cast j1 j2 ih1 ih2 =>
+  --   apply cast
+  --   apply ih1 wf e
+  --   apply ih2 wf e
+  -- case refl j =>
+  --   apply refl
+  --   apply Kinding.drop_weaken_global n wf e j
+  -- case sym j ih =>
+  --   apply sym
+  --   apply ih wf e
+  -- case seq j1 j2 ih1 ih2 =>
+  --   apply seq
+  --   apply ih1 wf e
+  --   apply ih2 wf e
+  -- case appc j1 j2 ih1 ih2 =>
+  --   apply appc
+  --   apply ih1 wf e
+  --   apply ih2 wf e
+  -- case arrowc j1 j2 ih1 ih2 =>
+  --   apply arrowc
+  --   apply ih1 wf e
+  --   apply ih2 wf e
+  -- case fst j1 j2 j3 ih =>
+  --   apply fst
+  --   apply Kinding.drop_weaken_global n wf e j1
+  --   apply Kinding.drop_weaken_global n wf e j2
+  --   apply ih wf e
+  -- case snd j1 j2 j3 ih =>
+  --   apply snd
+  --   apply Kinding.drop_weaken_global n wf e j1
+  --   apply Kinding.drop_weaken_global n wf e j2
+  --   apply ih wf e
+  -- case allc j ih =>
+  --   apply allc
+  --   apply ih wf e
+  -- case apptc j1 j2 j3 j4 ih1 ih2 =>
+  --   apply apptc
+  --   apply ih1 wf e
+  --   apply ih2 wf e
+  --   apply j3
+  --   apply j4
+  -- case zero j =>
+  --   apply zero
+  --   apply Kinding.drop_weaken_global n wf e j
+  -- case choice j1 j2 j3 ih1 ih2 =>
+  --   apply choice
+  --   apply Kinding.drop_weaken_global n wf e j1
+  --   apply ih1 wf e
+  --   apply ih2 wf e
+
+-- theorem GlobalWf.lookup_weaken :
+--   ⊢ (e1::G) ->
+--   lookup x G = some e2 ->
+--   lookup x (e1::G) = some e2
+-- := by
+--   intro wf j
+--   apply drop_lookup_unique 1 wf
+--   simp; exact j
+
+-- theorem EntryWf.weaken :
+--   ⊢ (e1::G) ->
+--   EntryWf G e2 ->
+--   EntryWf (e1::G) e2
+-- := by
+--   intro wf j
+--   induction j
+--   case data j =>
+--     apply EntryWf.data
+--     apply GlobalWf.lookup_weaken wf j
+--   case ctor j1 j2 j3 j4 j5 =>
+--     apply EntryWf.ctor
+--     apply GlobalWf.lookup_weaken wf j1
+--     apply j2
+--     apply Kinding.drop_weaken_global 1 wf (by simp) j3
+--     exact j4
+--     apply GlobalWf.lookup_weaken wf j5
+--   case opent j1 j2 =>
+--     apply EntryWf.opent j1
+--     apply GlobalWf.lookup_weaken wf j2
+--   case openm j1 j2 =>
+--     apply EntryWf.openm
+--     apply Kinding.drop_weaken_global 1 wf (by simp) j1
+--     apply GlobalWf.lookup_weaken wf j2
+--   case defn j1 j2 j3 j4 =>
+--     apply EntryWf.defn
+--     apply Kinding.drop_weaken_global 1 wf (by simp) j2
+--     apply Typing.drop_weaken_global 1 wf (by simp) j3
+--     apply GlobalWf.lookup_weaken wf j4
+--   case instty j1 j2 =>
+--     apply EntryWf.instty
+--     apply ValidInstTy.drop_weaken_global 1 wf (by simp) j1
+--     apply GlobalWf.lookup_weaken wf j2
+
+-- theorem EntryWf.from_lookup_vec1 :
+--   Vect.fold d Option.or v = some t ->
+--   (∃ i, v i = some t) ∨ d = some t
+-- := by
+--   intro h
+--   induction v using Vect.induction
+--   case nil => simp at *; exact h
+--   case cons hd tl ih =>
+--     simp at h; rcases h with h | ⟨h1, h2⟩
+--     subst h; apply Or.inl; exists 0
+--     subst h1; replace ih := ih h2
+--     cases ih
+--     case _ ih =>
+--       obtain ⟨i, ih⟩ := ih
+--       apply Or.inl; exists (Fin.succ i)
+--     case _ ih => apply Or.inr ih
+
+-- theorem EntryWf.from_lookup_vec2 :
+--   (∃ i, v i = some t ∧ (∀ j ≠ i, v j = none)) ->
+--   Vect.fold none Option.or v = some t
+-- := by
+--   intro h
+--   obtain ⟨i, h1, h2⟩ := h
+--   induction v using Vect.induction
+--   case nil =>
+--     exfalso; apply Fin.elim0 i
+--   case cons hd tl ih =>
+--     cases i using Fin.cases <;> simp at *
+--     case zero => apply Or.inl h1
+--     case succ i =>
+--       have h3 := λ j => h2 (Fin.succ j); simp at h3
+--       replace ih := ih i h1 h3
+--       apply Or.inr; apply And.intro _ ih
+--       apply h2 0; intro h; cases h
+
+-- theorem EntryWf.from_lookup_vec3 :
+--   (∀ i, v i = none) ->
+--   Vect.fold d Option.or v = d
+-- := by
+--   intro h
+--   induction v using Vect.induction
+--   case nil => simp
+--   case cons hd tl ih =>
+--     have lem1 := h 0; simp at lem1
+--     have lem2 := λ i => h (Fin.succ i); simp at lem2
+--     simp; rw [lem1, ih lem2]; simp
+
+-- theorem Kinding.global_weaken_ctors :
+--   (∀ x, (lookup_kind G x).isSome -> lookup_kind G x = lookup_kind G' x) ->
+--   G&Δ ⊢ T : K ->
+--   G'&Δ ⊢ T : K
+-- := by
+--   intro h j
+--   induction j generalizing G'
+--   case var j => apply var j
+--   case global x K Δ j =>
+--     apply global
+--     rw [<-h x]; apply j
+--     rw [j]; simp
+--   case arrow ih1 ih2 => apply arrow (ih1 h) (ih2 h)
+--   case all ih => apply all (ih h)
+--   case app ih1 ih2 => apply app (ih1 h) (ih2 h)
+--   case eq ih1 ih2 => apply eq (ih1 h) (ih2 h)
+
+-- theorem lookup_head_eq :
+--   lookup x (e1::G) = some e2 ->
+
+
+theorem EntryWf.lookup_defn
+  : lookup x G = some (.defn x A t) -> ⊢ G -> EntryWf G (.defn x A t)
+| h, .nil => sorry
+| h, .cons (.data j1 j2 j3) wf => sorry
+| h, .cons (.odata j1) wf => sorry
+| h, .cons (.openm j1 j2) wf =>
+  .defn sorry sorry h
+| h, .cons (.defn j1 j2 j3) wf => sorry
+| h, .cons (.inst j1 e j2 j3) wf => sorry
+| h, .cons (.octor j1 j2) wf => sorry
+
+theorem EntryWf.from_lookup (h : lookup x G = some e) : ⊢ G -> EntryWf G e
+| .nil => sorry
+| .cons (.data j1 j2 j3) wf => sorry
+| .cons (.odata j1) wf => sorry
+| .cons (.openm j1 j2) wf => sorry
+| .cons (.defn j1 j2 j3) wf => sorry
+| .cons (.inst j1 e j2 j3) wf => sorry
+| .cons (.octor j1 j2) wf => sorry
+
+theorem EntryWf.from_lookup2 :
+  ⊢ G ->
+  lookup x G = some e ->
+  EntryWf G e
+:= by
+  intro wf h
+  fun_induction lookup
+  case _ => sorry
+  case _ => sorry
+  case _ => sorry
+  case _ => sorry
+  case _ => sorry
+  case _ => sorry
+  case _ => sorry
+  case _ => sorry
+  case _ => sorry
+  case _ => sorry
+  case _ => sorry
+  case _ => sorry
+--   intro wf h
+--   induction wf generalizing e
+--   case nil => simp [lookup] at h
+--   case cons G g gwf wf ih =>
+--     have gwf' := gwf
+--     have wf' := ListGlobalWf.cons gwf' wf
+--     cases gwf <;> simp [lookup] at h
+--     case data dx K ctors j1 j2 j3 =>
+--       split at h
+--       case _ e1 =>
+--         subst e1; injection h with e; subst e
+--         apply EntryWf.data; simp [lookup]
+--       case _ e1 =>
+--         replace h := from_lookup_vec1 h
+--         rcases h with ⟨i, h⟩ | h
+--         case _ =>
+--           simp at h; obtain ⟨h1, h2⟩ := h
+--           rw [<-h2]
+--           generalize zdef : ctors i = z at *
+--           rcases z with ⟨z, zA⟩
+--           simp at *; subst h1
+--           obtain ⟨q1, q2, q3, q4⟩ := j2 i x zA zdef
+--           apply EntryWf.ctor dx K ctors; simp [lookup]
+--           exact zdef
+--           apply Kinding.global_weaken_ctors _ q1
+--           case _ =>
+--             intro x h
+--             unfold is_data at h
+--             simp [lookup_kind, lookup] at *
+--             split; simp [Entry.kind]
+--             split at h; case _ h1 h2 => exfalso; apply h1 h2
+--             rw [from_lookup_vec3]; intro i
+--             generalize wdef : ctors i = w
+--             cases w; case _ w wA =>
+--             simp; intro h; subst h
+--             obtain ⟨w1, w2, w3, w4⟩ := j2 i x wA wdef
+--             rw [w4] at h; simp [Option.isSome] at h
+--           exact q2; simp [lookup]
+--           split; case _ e => exfalso; apply e1 e
+--           case _ e =>
+--             rw [q4]
+--             apply from_lookup_vec2
+--             exists i; rw [zdef]; simp
+--             intro j w1 w2; apply j1 i j
+--             rw [<-w2, zdef]
+--         case _ => apply weaken wf' (ih h)
+--     case opent j1 j2 =>
+--       split at h
+--       case _ e1 =>
+--         subst e1; injection h with e; subst e
+--         apply EntryWf.opent j1; simp [lookup]
+--       case _ e1 => apply weaken wf' (ih h)
+--     case openm j1 j2 =>
+--       split at h
+--       case _ e1 =>
+--         subst e1; injection h with e; subst e
+--         apply EntryWf.openm
+--         apply Kinding.drop_weaken_global 1 wf' (by simp) j1
+--         simp [lookup]
+--       case _ e1 => apply weaken wf' (ih h)
+--     case defn j1 j2 j3 =>
+--       split at h
+--       case _ e1 =>
+--         subst e1; injection h with e; subst e
+--         apply EntryWf.defn
+--         apply Kinding.drop_weaken_global 1 wf' (by simp) j1
+--         apply Typing.drop_weaken_global 1 wf' (by simp) j2
+--         simp [lookup]
+--       case _ e1 => apply weaken wf' (ih h)
+--     case inst y T t j1 j2 =>
+--       replace ih := ih h
+--       apply weaken wf' ih
+--     case instty j1 j2 =>
+--       split at h
+--       case _ e1 =>
+--         subst e1; injection h with e; subst e
+--         apply EntryWf.instty
+--         apply ValidInstTy.drop_weaken_global 1 wf' (by simp) j1
+--         simp [lookup]
+--       case _ e1 => apply weaken wf' (ih h)
+
+-- theorem EntryWf.get_openm {G} {Δ} {Γ} :
+--   ⊢ G ->
+--   EntryWf G (.openm x T) ->
+--   G&Δ, Γ  ⊢ g#x : T ∧
+--   ∃ b, G&Δ ⊢ T : .base b
+-- := by
+--   intro wf e; cases e; case _ b j1 j2 =>
+--   apply And.intro
+--   apply Typing.global; simp [lookup_type]; rw [j2]; simp
+--   simp [Entry.type]
+--   apply Kinding.closed_arbitrary_weakening Δ wf j1
+--   exists b; apply Kinding.closed_arbitrary_weakening Δ wf j1
+
+-- theorem GlobalWf.types_have_base_kind :
+--   ⊢ G ->
+--   lookup_type G x = some T ->
+--   ∃ b, G&Δ ⊢ T : .base b
+-- := by
+--   intro wf h
+--   simp [lookup_type] at h
+--   generalize zdef : lookup x G = z at h
+--   cases z; simp at h; case _ z =>
+--   have lem := EntryWf.from_lookup wf zdef
+--   cases lem <;> simp [Entry.type] at h
+--   case ctor j1 j2 j3 j4 j5 =>
+--     apply Exists.intro _; subst h
+--     apply Kinding.closed_arbitrary_weakening Δ wf j4
+--   case openm j1 j2 =>
+--     apply Exists.intro _; subst h
+--     apply Kinding.closed_arbitrary_weakening Δ wf j1
+--   case defn j1 j2 j3 =>
+--     apply Exists.intro _; subst h
+--     apply Kinding.closed_arbitrary_weakening Δ wf j1
+--   case instty j1 j2 =>
+--     obtain ⟨b, lem⟩ := ValidInstTy.closed j1
+--     subst h; exists b
+--     apply Kinding.closed_arbitrary_weakening Δ wf lem
+
+-- theorem GlobalWf.lookup_type_sound :
+--   ⊢ G ->
+--   lookup_type G x = some T ->
+--   G&Δ,Γ ⊢ g#x : T := by
+--  intro wf h
+--  have lem := GlobalWf.types_have_base_kind (Δ := Δ) wf h;
+--  rcases lem with ⟨bk, lem⟩
+--  constructor; assumption;
+--  apply lem;
+
+-- theorem GlobalWf.lookup_defn_type_exists {G : List Global} {Δ : List Kind} :
+--   ⊢ G ->
+--   lookup_defn G x = some t ->
+--   ∃ T b, lookup_type G x = some T ∧ G&Δ ⊢ T : .base b
+-- := by
+--   intro wf h
+--   unfold lookup_defn at h; simp at h
+--   obtain ⟨w, q1, q2⟩ := Option.bind_eq_some_iff.1 h; clear h
+--   cases w <;> simp at q2; case _ y A t' =>
+--   subst q2
+--   have lem : lookup_type G x = some A := by
+--     simp [lookup_type]; rw [q1]; simp [Entry.type]
+--   obtain ⟨b, h⟩ := types_have_base_kind (Δ := Δ) wf lem
+--   exists A; exists b
+
+-- theorem GlobalWf.lookup_defn_type {G : List Global} {Δ : List Kind} {Γ : List Ty} :
+--   ⊢ G ->
+--   lookup_defn G x = some t ->
+--   ∃ T b, G&Δ,Γ ⊢ g#x : T ∧ G&Δ,Γ ⊢ t : T ∧ G&Δ ⊢ T : .base b
+-- := by
+--   intro wf j
+--   unfold lookup_defn at j; simp at j
+--   obtain ⟨a, j1, j2⟩ := Option.bind_eq_some_iff.1 j; clear j
+--   have lem := EntryWf.from_lookup wf j1
+--   cases lem <;> simp at j2
+--   case _ T b t y q1 q2 q3 =>
+--   subst j2; exists T; exists b; apply And.intro
+--   apply Typing.global; simp [lookup_type]; rw [j1]; simp [Entry.type]
+--   apply Kinding.closed_arbitrary_weakening Δ wf q1
+--   apply And.intro
+--   replace q2 := Typing.weaken_type_closed Δ wf q2
+--   apply Typing.weaken_closed Γ wf q2
+--   apply Kinding.closed_arbitrary_weakening Δ wf q1
+
+end Core
